src/extern/dotnet/StandardLibrary.cs
@@ -1,7 +1,7 @@
 namespace STL {
 
   public partial class __default {
-    public static Option<T> As<T>(object x) where T : class {
+    public static Option<T> Cast<T>(object x) where T : class {
       var casted = x as T;
       if (casted != null) {
         return Option<T>.create_Some(casted);
